Brought the Featherweight comparison into exactly the form that is given in their theories.

thy/OpenFlow/FeatherweightOpenFlowComparison.thy
@@ -3,21 +3,33 @@ imports Semantics_OpenFlow
 begin
 
 (* compare to https://github.com/frenetic-lang/featherweight-openflow/blob/master/coq/OpenFlow/OpenFlowSemantics.v#L260 *)
-inductive guha_match :: "('m, 'p) field_matcher \<Rightarrow> ('m, 'a) flowtable \<Rightarrow> (('m, 'a) flow_entry_match) \<Rightarrow> 'p \<Rightarrow> bool" where
-"fe \<in> set ft \<Longrightarrow> \<gamma> (ofe_fields fe) p = True \<Longrightarrow> \<forall>fe' \<in> set ft. ofe_prio fe' > ofe_prio fe \<longrightarrow> \<gamma> (ofe_fields fe') p = False \<Longrightarrow> guha_match \<gamma> ft fe p"
+inductive guha_table_semantics :: "('m, 'p) field_matcher \<Rightarrow> ('m, 'a) flowtable \<Rightarrow> 'p \<Rightarrow> 'a option \<Rightarrow> bool" where
+"\<gamma> (ofe_fields fe) p = True \<Longrightarrow> 
+ \<forall>fe' \<in> set (ft1 @ ft2). ofe_prio fe' > ofe_prio fe \<longrightarrow> \<gamma> (ofe_fields fe') p = False \<Longrightarrow> 
+ guha_table_semantics \<gamma> (ft1 @ fe # ft2) p (Some (ofe_action fe))" |
+"\<forall>fe \<in> set ft. \<gamma> (ofe_fields fe) p = False \<Longrightarrow>
+ guha_table_semantics \<gamma> ft p None"
 
-(* so\<dots> there's the possibility for a flow table with two matching entries. yay\<dots>? *)
-lemma 
-	assumes "\<exists>ff1 ff2. ff1 \<noteq> ff2 \<and> \<gamma> ff1 p \<and> \<gamma> ff2 p"
-	shows "\<exists>ft fe1 fe2. fe1 \<noteq> fe2 \<and> guha_match \<gamma> ft fe1 p \<and> guha_match \<gamma> ft fe2 p"
+(* 
+so\<dots> there's the possibility for a flow table with two matching entries.
+I'm not so sure it is a good idea to model undefined behavior by nondeterministic but very defined behavior..
+*)
+lemma
+    assumes ta: "CARD('a) \<ge> 2" (* if there's only one action, the whole thing is moot. *)
+	assumes ms: "\<exists>ff. \<gamma> ff p" (* if our matcher rejects the packet for any match condition, it is borked. *)
+	shows "\<exists>ft (a1 :: 'a) (a2 :: 'a). a1 \<noteq> a2 \<and> guha_table_semantics \<gamma> ft p (Some a1) \<and> guha_table_semantics \<gamma> ft p (Some a2)"
 proof -
-	from assms 
-	obtain ff1 ff2 where ffs: "ff1 \<noteq> ff2" and m1: "\<gamma> ff1 p" and m2: "\<gamma> ff2 p" by (metis card2_eI mem_Collect_eq)
-	let ?fe1 = "OFEntry 0 ff1 undefined"
-	let ?fe2 = "OFEntry 0 ff2 undefined"
+	from ms	obtain ff  where m: "\<gamma> ff p" ..
+	from ta obtain a1 a2 :: 'a where as: "a1 \<noteq> a2" using card2_eI by blast
+	let ?fe1 = "OFEntry 0 ff a1"
+	let ?fe2 = "OFEntry 0 ff a2"
 	let ?ft = "[?fe1, ?fe2]"
-	have "guha_match \<gamma> ?ft ?fe1 p" "guha_match \<gamma> ?ft ?fe2 p" by(rule guha_match.intros; simp add: m1 m2)+
-	thus ?thesis using ffs by blast
+	find_theorems "_ @ [_]"
+	have "guha_table_semantics \<gamma> ?ft p (Some a1)" "guha_table_semantics \<gamma> ?ft p (Some a2)" 
+	by(rule guha_table_semantics.intros(1)[of \<gamma> ?fe1 p "[]" "[?fe2]", unfolded append_Nil flow_entry_match.sel] | 
+	   rule guha_table_semantics.intros(1)[of \<gamma> ?fe2 p "[?fe1]" "[]", unfolded append_Nil2 flow_entry_match.sel append.simps] |
+	   simp add: m)+
+	thus ?thesis using as by blast
 qed
 
 end
